implementing KDF

src/RIoT.X509.fst
@@ -138,8 +138,13 @@ let rec memcpy
   | 0ul -> ()
   | _   -> memcpy dst src cur
 
+assume val unit32_to_bigendian
+  (i: I.uint_32)
+: I.uint_32
+
+/// TODO
 #reset-options "--z3rlimit 50 --max_fuel 50 --max_ifuel 50"
-let riot_kdf_fixed
+let riot_KDF_FIXED
   (#fixed_size: I.uint_32{(v fixed_size) > 0})
   (fixed: B.lbuffer HI.uint8 (v fixed_size))
   (#label_size: I.uint_32{(v label_size) > 0})
@@ -176,32 +181,147 @@ let riot_kdf_fixed
 ///        fixed += labelSize;
 ///    }
   //memcpy fixed label label_size;
-  let fixed' = B.sub fixed 0ul label_size in
+  //let fixed' = B.sub fixed 0ul label_size in
 
 /// REF: *fixed++ = 0;
-  fixed'.(1ul) <- (HI.u8 0x00);
+  //fixed'.(1ul) <- (HI.u8 0x00);
 
 /// REF: if (context) {
 ///        memcpy(fixed, context, contextSize);
 ///        fixed += contextSize;
 ///      }
   //memcpy fixed' context context_size;
-  let fixed'' = B.sub fixed 0ul label_size in
+  //let fixed'' = B.sub fixed 0ul label_size in
 
 /// REF: numberOfBits = UINT32_TO_BIGENDIAN(numberOfBits);
-
+  let numberOfBits = unit32_to_bigendian numberOfBits in
 /// REF: memcpy(fixed, &numberOfBits, 4);
   //memcpy fixed''
 /// REF: return total;
 
   HST.pop_frame()
 
+type hashMagic_t = I.uint_64
+let _SHA256_BLOCK_LENGTH = block_len SHA2_256
+let _SHA256_DIGEST_LENGTH = hash_len SHA2_256
+let _HMAC_SHA256_BLOCK_LENGTH = block_len SHA2_256
+let _HMAC_SHA256_DIGEST_LENGTH = hash_len SHA2_256
+
+noeq
+type riot_SHA256_CONTEXT = {
+     state: B.lbuffer HI.uint8 8;
+     magic_: hashMagic_t;
+     bitcount: I.uint_64;
+     buffer: B.lbuffer HI.uint8 (v _SHA256_BLOCK_LENGTH)
+  }
+
+noeq
+type riot_HMAC_SHA256_CTX = {
+     hashCtx: riot_SHA256_CONTEXT;
+     opad: B.lbuffer HI.uint8 (v _HMAC_SHA256_BLOCK_LENGTH);
+  }
+
+#reset-options "--z3rlimit 50 --max_fuel 50 --max_ifuel 50"
+#push-options "--query_stats"
+let test
+  (a:I.uint_32)
+  (b:I.uint_32)
+  (c:B.pointer I.uint_32)
+: HST.Stack unit
+  (requires fun h ->
+      B.live h c
+    /\ I.ok (+) 1ul (B.get h c 0))
+  (ensures  fun h0 _ h1 -> True)
+=
+  let c : I.uint_32 = 1ul + !*c in
+  ()
+
+assume val riot_HMAC_SHA256_Init
+  (ctx: riot_HMAC_SHA256_CTX)
+  (#keyLen: I.uint_32{v keyLen > 0})
+  (key: B.lbuffer HI.uint8 (v keyLen))
+: HST.Stack unit
+  (requires fun h -> True)
+  (ensures  fun h0 _ h1 -> True)
+
+assume val riot_HMAC_SHA256_Update
+  (ctx: riot_HMAC_SHA256_CTX)
+  (#dataLen: I.uint_32{v dataLen > 0})
+  (data: B.lbuffer HI.uint8 (v dataLen))
+: HST.Stack unit
+  (requires fun h -> True)
+  (ensures  fun h0 _ h1 -> True)
+
+assume val riot_HMAC_SHA256_Final
+  (ctx: riot_HMAC_SHA256_CTX)
+  (#digestLen: I.uint_32{v digestLen > 0})
+  (digest: B.lbuffer HI.uint8 (v digestLen))
+: HST.Stack unit
+  (requires fun h -> True)
+  (ensures  fun h0 _ h1 -> True)
+
+let riot_KDF_SHA256
+  (#out_size: I.uint_32{v out_size > 0})
+  (out: B.lbuffer HI.uint8 (v out_size))
+  (#key_size: I.uint_32{v key_size > 0})
+  (key: B.lbuffer HI.uint8 (v key_size))
+  (#fixed_size: I.uint_32{v fixed_size > 0})
+  (fixed: B.lbuffer HI.uint8 (v fixed_size))
+  (counter: B.pointer HI.uint32)
+: HST.Stack unit
+  (requires fun h ->
+      B.live h counter
+    /\ B.live h out
+    /\ B.live h key
+    /\ B.disjoint counter out
+    /\ B.disjoint counter key
+    /\ B.disjoint key out
+    /\ I.ok (+) (B.get h counter 0) (HI.U32 1))
+  (ensures  fun h0 _ h1 -> True)
+=
+  HST.push_frame();
+
+/// REF: RIOT_HMAC_SHA256_CTX    ctx;
+  let ctx: riot_HMAC_SHA256_CTX = {
+      hashCtx = {
+        state = B.alloca (HI.u8 0x00) 8ul;
+        magic_ = 0uL;
+        bitcount = 0uL;
+        buffer = B.alloca (HI.u8 0x00) _SHA256_BLOCK_LENGTH
+      };
+      opad = B.alloca (HI.u8 0x00) _HMAC_SHA256_BLOCK_LENGTH
+  } in
+
+/// NOTE: Why `(!*counter) + 1ul` won't pass the type check?
+/// REF: uint32_t                ctr = counter ? ++*counter : 1;
+  let ctr: B.pointer HI.uint32
+    = B.alloca ((HI.u32 1) + !*counter) 1ul in
+
+  riot_HMAC_SHA256_Init
+    ctx
+    key;
+
+  riot_HMAC_SHA256_Update
+    ctx
+    ctr;
+
+  riot_HMAC_SHA256_Update
+    ctx
+    fixed;
+
+  riot_HMAC_SHA256_Final
+    ctx
+    out;
+
+  HST.pop_frame()
+
+
 let ecdh_derive
   (p1: affine_point_t)
   (k: bigval_t)
   (src: bigval_t)
   (label_size: I.uint_32)
-  (label: B.lbuffer uint8 (I.v label_size))
+  (label: B.lbuffer HI.uint8 (I.v label_size))
 : HST.Stack unit
   (requires fun h ->
       live_affine_point h p1
@@ -210,6 +330,6 @@ let ecdh_derive
 =
   HST.push_frame();
 
-  k.data.(1ul) <- (u32 0);
+  k.data.(_BIGLEN - 1ul) <- (HI.u32 0);
 
   HST.pop_frame()
